Source/Dafny/DafnyPrelude.bpl
@@ -81,13 +81,14 @@ axiom (forall t, u: Ty :: { TMap(t,u) }    Tag(TMap(t,u))    == TagMap);
 axiom (forall t, u: Ty :: { TIMap(t,u) }   Tag(TIMap(t,u))   == TagIMap);
 
 type TyTagFamily;
-function TagFamily(Ty): TyTagFamily;
+function {:exclude_dep} TagFamily(Ty): TyTagFamily;
 
 // ---------------------------------------------------------------
 // -- Literals ---------------------------------------------------
 // ---------------------------------------------------------------
-function {:identity} Lit<T>(x: T): T { x }
-axiom (forall<T> x: T :: { $Box(Lit(x)) } $Box(Lit(x)) == Lit($Box(x)) );
+function {:identity} {:exclude_dep} Lit<T>(x: T): T { x } uses {
+  axiom (forall<T> x: T :: { $Box(Lit(x)) } $Box(Lit(x)) == Lit($Box(x)) );
+}
 
 // Specialize Lit to concrete types.
 // These aren't logically required, but on some examples improve
@@ -191,113 +192,117 @@ axiom (forall<T> v : T, t : Ty, h : Heap ::
 
 // Type-argument to $Is is the /representation type/,
 // the second value argument to $Is is the actual type.
-function $Is<T>(T,Ty): bool;           // no heap for now
-function $IsAlloc<T>(T,Ty,Heap): bool;
+function {:exclude_dep} $Is<T>(T,Ty): bool uses {           // no heap for now
+    axiom(forall v : int  :: { $Is(v,TInt) }  $Is(v,TInt));
+    axiom(forall v : real :: { $Is(v,TReal) } $Is(v,TReal));
+    axiom(forall v : bool :: { $Is(v,TBool) } $Is(v,TBool));
+    axiom(forall v : char :: { $Is(v,TChar) } $Is(v,TChar));
+    axiom(forall v : ORDINAL :: { $Is(v,TORDINAL) } $Is(v,TORDINAL));
+    
+    // Since every bitvector type is a separate type in Boogie, the $Is/$IsAlloc axioms
+    // for bitvectors are generated programatically. Except, TBitvector(0) is given here.
+    axiom (forall v: Bv0 :: { $Is(v, TBitvector(0)) } $Is(v, TBitvector(0)));
+
+    axiom (forall v: Set Box, t0: Ty :: { $Is(v, TSet(t0)) }
+      $Is(v, TSet(t0)) <==>
+      (forall bx: Box :: { v[bx] }
+        v[bx] ==> $IsBox(bx, t0)));
+    axiom (forall v: ISet Box, t0: Ty :: { $Is(v, TISet(t0)) }
+      $Is(v, TISet(t0)) <==>
+      (forall bx: Box :: { v[bx] }
+        v[bx] ==> $IsBox(bx, t0)));
+    axiom (forall v: MultiSet Box, t0: Ty :: { $Is(v, TMultiSet(t0)) }
+      $Is(v, TMultiSet(t0)) <==>
+      (forall bx: Box :: { v[bx] }
+        0 < v[bx] ==> $IsBox(bx, t0)));
+    axiom (forall v: MultiSet Box, t0: Ty :: { $Is(v, TMultiSet(t0)) }
+      $Is(v, TMultiSet(t0)) ==> $IsGoodMultiSet(v));
+    axiom (forall v: Seq Box, t0: Ty :: { $Is(v, TSeq(t0)) }
+      $Is(v, TSeq(t0)) <==>
+      (forall i : int :: { Seq#Index(v, i) }
+        0 <= i && i < Seq#Length(v) ==>
+        $IsBox(Seq#Index(v, i), t0)));
+        
+    axiom (forall v: Map Box Box, t0: Ty, t1: Ty ::
+      { $Is(v, TMap(t0, t1)) }
+      $Is(v, TMap(t0, t1))
+         <==> (forall bx: Box ::
+          { Map#Elements(v)[bx] } { Map#Domain(v)[bx] }
+          Map#Domain(v)[bx] ==>
+            $IsBox(Map#Elements(v)[bx], t1) &&
+            $IsBox(bx, t0)));
+            
+    axiom (forall v: Map Box Box, t0: Ty, t1: Ty ::
+      { $Is(v, TMap(t0, t1)) }
+      $Is(v, TMap(t0, t1)) ==>
+        $Is(Map#Domain(v), TSet(t0)) &&
+        $Is(Map#Values(v), TSet(t1)) &&
+        $Is(Map#Items(v), TSet(Tclass._System.Tuple2(t0, t1))));
+    axiom (forall v: IMap Box Box, t0: Ty, t1: Ty ::
+      { $Is(v, TIMap(t0, t1)) }
+      $Is(v, TIMap(t0, t1))
+         <==> (forall bx: Box ::
+          { IMap#Elements(v)[bx] } { IMap#Domain(v)[bx] }
+          IMap#Domain(v)[bx] ==>
+            $IsBox(IMap#Elements(v)[bx], t1) &&
+            $IsBox(bx, t0)));
+    axiom (forall v: IMap Box Box, t0: Ty, t1: Ty ::
+      { $Is(v, TIMap(t0, t1)) }
+      $Is(v, TIMap(t0, t1)) ==>
+        $Is(IMap#Domain(v), TISet(t0)) &&
+        $Is(IMap#Values(v), TISet(t1)) &&
+        $Is(IMap#Items(v), TISet(Tclass._System.Tuple2(t0, t1))));
+}
+function {:exclude_dep}  $IsAlloc<T>(T,Ty,Heap): bool uses {
+    axiom(forall h : Heap, v : int  :: { $IsAlloc(v,TInt,h) }  $IsAlloc(v,TInt,h));
+    axiom(forall h : Heap, v : real :: { $IsAlloc(v,TReal,h) } $IsAlloc(v,TReal,h));
+    axiom(forall h : Heap, v : bool :: { $IsAlloc(v,TBool,h) } $IsAlloc(v,TBool,h));
+    axiom(forall h : Heap, v : char :: { $IsAlloc(v,TChar,h) } $IsAlloc(v,TChar,h));
+    axiom(forall h : Heap, v : ORDINAL :: { $IsAlloc(v,TORDINAL,h) } $IsAlloc(v,TORDINAL,h));
+    
+    axiom (forall v: Bv0, h: Heap :: { $IsAlloc(v, TBitvector(0), h) } $IsAlloc(v, TBitvector(0), h));
+    
+    axiom (forall v: Set Box, t0: Ty, h: Heap :: { $IsAlloc(v, TSet(t0), h) }
+      $IsAlloc(v, TSet(t0), h) <==>
+      (forall bx: Box :: { v[bx] }
+        v[bx] ==> $IsAllocBox(bx, t0, h)));
+    axiom (forall v: ISet Box, t0: Ty, h: Heap :: { $IsAlloc(v, TISet(t0), h) }
+      $IsAlloc(v, TISet(t0), h) <==>
+      (forall bx: Box :: { v[bx] }
+        v[bx] ==> $IsAllocBox(bx, t0, h)));
+    axiom (forall v: MultiSet Box, t0: Ty, h: Heap :: { $IsAlloc(v, TMultiSet(t0), h) }
+      $IsAlloc(v, TMultiSet(t0), h) <==>
+      (forall bx: Box :: { v[bx] }
+        0 < v[bx] ==> $IsAllocBox(bx, t0, h)));
+    axiom (forall v: Seq Box, t0: Ty, h: Heap :: { $IsAlloc(v, TSeq(t0), h) }
+      $IsAlloc(v, TSeq(t0), h) <==>
+      (forall i : int :: { Seq#Index(v, i) }
+        0 <= i && i < Seq#Length(v) ==>
+    	$IsAllocBox(Seq#Index(v, i), t0, h)));
+    	
+    axiom (forall v: Map Box Box, t0: Ty, t1: Ty, h: Heap ::
+      { $IsAlloc(v, TMap(t0, t1), h) }
+      $IsAlloc(v, TMap(t0, t1), h)
+         <==> (forall bx: Box ::
+          { Map#Elements(v)[bx] } { Map#Domain(v)[bx] }
+          Map#Domain(v)[bx] ==>
+            $IsAllocBox(Map#Elements(v)[bx], t1, h) &&
+            $IsAllocBox(bx, t0, h)));
+            
+    axiom (forall v: IMap Box Box, t0: Ty, t1: Ty, h: Heap ::
+      { $IsAlloc(v, TIMap(t0, t1), h) }
+      $IsAlloc(v, TIMap(t0, t1), h)
+         <==> (forall bx: Box ::
+          { IMap#Elements(v)[bx] } { IMap#Domain(v)[bx] }
+          IMap#Domain(v)[bx] ==>
+            $IsAllocBox(IMap#Elements(v)[bx], t1, h) &&
+            $IsAllocBox(bx, t0, h)));
+}
 
 // Corresponding entries for boxes...
 // This could probably be solved by having Box also inhabit Ty
 function $IsBox<T>(T,Ty): bool;
 function $IsAllocBox<T>(T,Ty,Heap): bool;
-
-axiom(forall v : int  :: { $Is(v,TInt) }  $Is(v,TInt));
-axiom(forall v : real :: { $Is(v,TReal) } $Is(v,TReal));
-axiom(forall v : bool :: { $Is(v,TBool) } $Is(v,TBool));
-axiom(forall v : char :: { $Is(v,TChar) } $Is(v,TChar));
-axiom(forall v : ORDINAL :: { $Is(v,TORDINAL) } $Is(v,TORDINAL));
-
-axiom(forall h : Heap, v : int  :: { $IsAlloc(v,TInt,h) }  $IsAlloc(v,TInt,h));
-axiom(forall h : Heap, v : real :: { $IsAlloc(v,TReal,h) } $IsAlloc(v,TReal,h));
-axiom(forall h : Heap, v : bool :: { $IsAlloc(v,TBool,h) } $IsAlloc(v,TBool,h));
-axiom(forall h : Heap, v : char :: { $IsAlloc(v,TChar,h) } $IsAlloc(v,TChar,h));
-axiom(forall h : Heap, v : ORDINAL :: { $IsAlloc(v,TORDINAL,h) } $IsAlloc(v,TORDINAL,h));
-
-// Since every bitvector type is a separate type in Boogie, the $Is/$IsAlloc axioms
-// for bitvectors are generated programatically. Except, TBitvector(0) is given here.
-axiom (forall v: Bv0 :: { $Is(v, TBitvector(0)) } $Is(v, TBitvector(0)));
-axiom (forall v: Bv0, h: Heap :: { $IsAlloc(v, TBitvector(0), h) } $IsAlloc(v, TBitvector(0), h));
-
-axiom (forall v: Set Box, t0: Ty :: { $Is(v, TSet(t0)) }
-  $Is(v, TSet(t0)) <==>
-  (forall bx: Box :: { v[bx] }
-    v[bx] ==> $IsBox(bx, t0)));
-axiom (forall v: ISet Box, t0: Ty :: { $Is(v, TISet(t0)) }
-  $Is(v, TISet(t0)) <==>
-  (forall bx: Box :: { v[bx] }
-    v[bx] ==> $IsBox(bx, t0)));
-axiom (forall v: MultiSet Box, t0: Ty :: { $Is(v, TMultiSet(t0)) }
-  $Is(v, TMultiSet(t0)) <==>
-  (forall bx: Box :: { v[bx] }
-    0 < v[bx] ==> $IsBox(bx, t0)));
-axiom (forall v: MultiSet Box, t0: Ty :: { $Is(v, TMultiSet(t0)) }
-  $Is(v, TMultiSet(t0)) ==> $IsGoodMultiSet(v));
-axiom (forall v: Seq Box, t0: Ty :: { $Is(v, TSeq(t0)) }
-  $Is(v, TSeq(t0)) <==>
-  (forall i : int :: { Seq#Index(v, i) }
-    0 <= i && i < Seq#Length(v) ==>
-	$IsBox(Seq#Index(v, i), t0)));
-axiom (forall v: Set Box, t0: Ty, h: Heap :: { $IsAlloc(v, TSet(t0), h) }
-  $IsAlloc(v, TSet(t0), h) <==>
-  (forall bx: Box :: { v[bx] }
-    v[bx] ==> $IsAllocBox(bx, t0, h)));
-axiom (forall v: ISet Box, t0: Ty, h: Heap :: { $IsAlloc(v, TISet(t0), h) }
-  $IsAlloc(v, TISet(t0), h) <==>
-  (forall bx: Box :: { v[bx] }
-    v[bx] ==> $IsAllocBox(bx, t0, h)));
-axiom (forall v: MultiSet Box, t0: Ty, h: Heap :: { $IsAlloc(v, TMultiSet(t0), h) }
-  $IsAlloc(v, TMultiSet(t0), h) <==>
-  (forall bx: Box :: { v[bx] }
-    0 < v[bx] ==> $IsAllocBox(bx, t0, h)));
-axiom (forall v: Seq Box, t0: Ty, h: Heap :: { $IsAlloc(v, TSeq(t0), h) }
-  $IsAlloc(v, TSeq(t0), h) <==>
-  (forall i : int :: { Seq#Index(v, i) }
-    0 <= i && i < Seq#Length(v) ==>
-	$IsAllocBox(Seq#Index(v, i), t0, h)));
-
-axiom (forall v: Map Box Box, t0: Ty, t1: Ty ::
-  { $Is(v, TMap(t0, t1)) }
-  $Is(v, TMap(t0, t1))
-     <==> (forall bx: Box ::
-      { Map#Elements(v)[bx] } { Map#Domain(v)[bx] }
-      Map#Domain(v)[bx] ==>
-        $IsBox(Map#Elements(v)[bx], t1) &&
-        $IsBox(bx, t0)));
-axiom (forall v: Map Box Box, t0: Ty, t1: Ty, h: Heap ::
-  { $IsAlloc(v, TMap(t0, t1), h) }
-  $IsAlloc(v, TMap(t0, t1), h)
-     <==> (forall bx: Box ::
-      { Map#Elements(v)[bx] } { Map#Domain(v)[bx] }
-      Map#Domain(v)[bx] ==>
-        $IsAllocBox(Map#Elements(v)[bx], t1, h) &&
-        $IsAllocBox(bx, t0, h)));
-axiom (forall v: Map Box Box, t0: Ty, t1: Ty ::
-  { $Is(v, TMap(t0, t1)) }
-  $Is(v, TMap(t0, t1)) ==>
-    $Is(Map#Domain(v), TSet(t0)) &&
-    $Is(Map#Values(v), TSet(t1)) &&
-    $Is(Map#Items(v), TSet(Tclass._System.Tuple2(t0, t1))));
-
-axiom (forall v: IMap Box Box, t0: Ty, t1: Ty ::
-  { $Is(v, TIMap(t0, t1)) }
-  $Is(v, TIMap(t0, t1))
-     <==> (forall bx: Box ::
-      { IMap#Elements(v)[bx] } { IMap#Domain(v)[bx] }
-      IMap#Domain(v)[bx] ==>
-        $IsBox(IMap#Elements(v)[bx], t1) &&
-        $IsBox(bx, t0)));
-axiom (forall v: IMap Box Box, t0: Ty, t1: Ty, h: Heap ::
-  { $IsAlloc(v, TIMap(t0, t1), h) }
-  $IsAlloc(v, TIMap(t0, t1), h)
-     <==> (forall bx: Box ::
-      { IMap#Elements(v)[bx] } { IMap#Domain(v)[bx] }
-      IMap#Domain(v)[bx] ==>
-        $IsAllocBox(IMap#Elements(v)[bx], t1, h) &&
-        $IsAllocBox(bx, t0, h)));
-axiom (forall v: IMap Box Box, t0: Ty, t1: Ty ::
-  { $Is(v, TIMap(t0, t1)) }
-  $Is(v, TIMap(t0, t1)) ==>
-    $Is(IMap#Domain(v), TISet(t0)) &&
-    $Is(IMap#Values(v), TISet(t1)) &&
-    $Is(IMap#Items(v), TISet(Tclass._System.Tuple2(t0, t1))));
 
 // ---------------------------------------------------------------
 // -- Encoding of type names -------------------------------------
@@ -344,7 +349,7 @@ function Apply1(Ty, Ty, Heap, HandleType, Box): Box;
 type DatatypeType;
 
 type DtCtorId;
-function DatatypeCtorId(DatatypeType): DtCtorId;
+function {:exclude_dep} DatatypeCtorId(DatatypeType): DtCtorId;
 
 function DtRank(DatatypeType): int;
 function BoxRank(Box): int;
@@ -447,7 +452,7 @@ axiom (forall o: ORDINAL, m,n: int ::
 
 // used to make sure function axioms are not used while their consistency is being checked
 const $ModuleContextHeight: int;
-const $FunctionContextHeight: int;
+const {:exclude_dep} $FunctionContextHeight: int;
 
 // ---------------------------------------------------------------
 // -- Layers of function encodings -------------------------------
@@ -468,7 +473,7 @@ axiom (forall<A> f : [LayerType]A, ly : LayerType :: { AtLayer(f,$LS(ly)) } AtLa
 
 type Field alpha;
 
-function FDim<T>(Field T): int;
+function {:exclude_dep} FDim<T>(Field T): int;
 
 function IndexField(int): Field Box;
 axiom (forall i: int :: { IndexField(i) } FDim(IndexField(i)) == 1);
@@ -492,7 +497,9 @@ axiom (forall<T> cl : ClassName, nm: NameFamily ::
    {FieldOfDecl(cl, nm): Field T}
    DeclType(FieldOfDecl(cl, nm): Field T) == cl && DeclName(FieldOfDecl(cl, nm): Field T) == nm);
 
-function $IsGhostField<T>(Field T): bool;
+function {:exclude_dep} $IsGhostField<T>(Field T): bool uses {
+  axiom !$IsGhostField(alloc); // treat as non-ghost field, because it cannot be changed by ghost code
+}
 
 // ---------------------------------------------------------------
 // -- Allocatedness and Heap Succession --------------------------
@@ -513,8 +520,7 @@ axiom(forall h, k : Heap, bx : Box, t : Ty ::
 const unique alloc: Field bool;
 const unique allocName: NameFamily;
 axiom FDim(alloc) == 0 &&
-  DeclName(alloc) == allocName &&
-  $IsGhostField(alloc);  // treat as ghost field, since it is allowed to be changed by ghost code
+  DeclName(alloc) == allocName;
 
 // ---------------------------------------------------------------
 // -- Arrays -----------------------------------------------------
